tests/layeff/LowParseWriters.Parsers.fsti
@@ -14,7 +14,7 @@ val get_parser_kind
 
 val get_parser
   (p: parser)
-: Tot (LP.parser (get_parser_kind p) (dfst p))
+: Tot (LP.parser (get_parser_kind p) (Parser?.t p))
 
 val get_serializer
   (p: parser)
@@ -39,7 +39,7 @@ let make_parser
   (s: LP.serializer p)
   (j: LP.jumper p)
 : Tot parser
-= (| t, make_parser' p s j |)
+= Parser t (make_parser' p s j)
 
 val make_parser_correct
   (#t: Type)
@@ -57,7 +57,7 @@ val make_parser_correct
 
 val size_correct
   (p: parser)
-  (x: dfst p)
+  (x: Parser?.t p)
 : Lemma
   (size p x == Seq.length (LP.serialize (get_serializer p) x))
   [SMTPat (size p x)]
@@ -74,7 +74,7 @@ let deref
   (#inv: memory_invariant)
   (r: LP.leaf_reader (get_parser p))
   (x: ptr p inv)
-: Read (dfst p) True (fun res -> res == deref_spec x) inv
+: Read (Parser?.t p) True (fun res -> res == deref_spec x) inv
 = deref (leaf_reader_of_lp_leaf_reader p r) x
 
 inline_for_extraction
@@ -92,7 +92,7 @@ let start
     (get_parser_kind p).LP.parser_kind_high == Some (get_parser_kind p).LP.parser_kind_low
   })
   (#l: memory_invariant)
-  (x: dfst p)
+  (x: Parser?.t p)
 : Write unit emp (p) (fun _ -> True) (fun _ _ y -> y == x) l
 = start (leaf_writer_of_lp_leaf_writer p w) x
 
@@ -104,14 +104,14 @@ let append
     (get_parser_kind p).LP.parser_kind_high == Some (get_parser_kind p).LP.parser_kind_low
   })
   (#l: memory_invariant)
-  (x: dfst p)
+  (x: Parser?.t p)
 : Write unit fr (fr `star` p) (fun _ -> True) (fun w _ (w', x') -> w' == w /\ x' == x) l
 = append (leaf_writer_of_lp_leaf_writer p w) x
 
 inline_for_extraction
 let access_t
   (p1 p2: parser)
-  (#lens: LP.clens (dfst p1) (dfst p2))
+  (#lens: LP.clens (Parser?.t p1) (Parser?.t p2))
   (#g: LP.gaccessor (get_parser p1) (get_parser p2) lens)
   (a: LP.accessor g)
 : Tot Type
@@ -122,7 +122,7 @@ let access_t
 
 val access_spec
   (p1 p2: parser)
-  (#lens: LP.clens (dfst p1) (dfst p2))
+  (#lens: LP.clens (Parser?.t p1) (Parser?.t p2))
   (#g: LP.gaccessor (get_parser p1) (get_parser p2) lens)
   (a: LP.accessor g)
   (#inv: memory_invariant)
@@ -134,7 +134,7 @@ val access_spec
 inline_for_extraction
 val access_impl
   (p1 p2: parser)
-  (#lens: LP.clens (dfst p1) (dfst p2))
+  (#lens: LP.clens (Parser?.t p1) (Parser?.t p2))
   (#g: LP.gaccessor (get_parser p1) (get_parser p2) lens)
   (a: LP.accessor g)
   (#inv: memory_invariant)
@@ -144,7 +144,7 @@ val access_impl
 inline_for_extraction
 let access
   (p1 p2: parser)
-  (#lens: LP.clens (dfst p1) (dfst p2))
+  (#lens: LP.clens (Parser?.t p1) (Parser?.t p2))
   (#g: LP.gaccessor (get_parser p1) (get_parser p2) lens)
   (a: LP.accessor g)
 : Tot (access_t p1 p2 a)
@@ -154,9 +154,9 @@ let access
 val valid_synth_parser_eq
   (p1: parser)
   (p2: parser {
-    dfst p1 == dfst p2 /\
+    Parser?.t p1 == Parser?.t p2 /\
     get_parser_kind p1 == get_parser_kind p2 /\
-    get_parser p1 == LP.coerce (LP.parser (get_parser_kind p1) (dfst p1)) (get_parser p2)
+    get_parser p1 == LP.coerce (LP.parser (get_parser_kind p1) (Parser?.t p1)) (get_parser p2)
   })
 : Tot (valid_synth_t p1 p2 (fun _ -> True) (fun x -> x))
 
@@ -164,7 +164,7 @@ let parse_vldata_pred
   (min: nat)
   (max: nat)
   (p: parser)
-  (x: dfst p)
+  (x: Parser?.t p)
 : GTot Type0
 = let reslen = size p x in
   min <= reslen /\ reslen <= max
@@ -174,7 +174,7 @@ let parse_vldata_t
   (max: nat)
   (p: parser)
 : Tot Type
-= (x: dfst p { parse_vldata_pred min max p x } )
+= (x: Parser?.t p { parse_vldata_pred min max p x } )
 
 inline_for_extraction
 val parse_vldata
@@ -182,7 +182,7 @@ val parse_vldata
   (min: U32.t)
   (max: U32.t { U32.v min <= U32.v max /\ U32.v max > 0 })
 : Tot (p' : parser {
-    dfst p' == parse_vldata_t (U32.v min) (U32.v max) p
+    Parser?.t p' == parse_vldata_t (U32.v min) (U32.v max) p
   })
 
 inline_for_extraction
@@ -225,7 +225,7 @@ inline_for_extraction
 val parse_bounded_integer
   (sz: integer_size)
 : Tot (p' : parser {
-    dfst p' == LPI.bounded_integer (U32.v sz) /\
+    Parser?.t p' == LPI.bounded_integer (U32.v sz) /\
     get_parser_kind p' == LPI.parse_bounded_integer_kind (U32.v sz) /\
     get_parser p' == LPI.parse_bounded_integer (U32.v sz) /\
     get_serializer p' == LPI.serialize_bounded_integer (U32.v sz)
@@ -256,7 +256,7 @@ let parse_vldata_intro
 : Write unit (parse_bounded_integer (log256 max) `star` p) (parse_vldata p min max)
   (fun (_, vin) -> U32.v min <= size p vin /\ size p vin <= U32.v max)
   (fun (_, vin) _ vout -> vin == vout) inv
-= EWrite?.reflect (| parse_vldata_intro_spec p min max, parse_vldata_intro_impl p min max |)
+= EWrite?.reflect (Repr (parse_vldata_intro_spec p min max) (parse_vldata_intro_impl p min max))
 
 inline_for_extraction
 val write_bounded_integer
@@ -287,7 +287,7 @@ let parse_vldata_intro_ho
       begin match destr_repr_spec _ _ _ _ _ _ _ f () with
       | Correct (_, v) ->
         post () () v /\
-        (vout <: dfst p) == v
+        (vout <: Parser?.t p) == v
       | _ -> False
       end
     )
@@ -336,7 +336,7 @@ let parse_vldata_intro_frame
   (p: parser)
   (min: U32.t)
   (max: U32.t { U32.v min <= U32.v max /\ U32.v max > 0 })
-: Write unit ((frame `star` parse_bounded_integer (log256 (max))) `star` p) (frame `star` parse_vldata p min max) (fun (_, vin) -> U32.v min <= size p vin /\ size p vin <= U32.v max) (fun ((fr, _), vin) _ (fr', vout) -> fr == fr' /\ (vin <: dfst p) == (vout <: dfst p)) inv
+: Write unit ((frame `star` parse_bounded_integer (log256 (max))) `star` p) (frame `star` parse_vldata p min max) (fun (_, vin) -> U32.v min <= size p vin /\ size p vin <= U32.v max) (fun ((fr, _), vin) _ (fr', vout) -> fr == fr' /\ (vin <: Parser?.t p) == (vout <: Parser?.t p)) inv
 = valid_synth _ _ _ _ _ (valid_synth_star_assoc_1 _ _ _);
   frame2 _ _ _ _ _ _ _ _ (fun _ -> parse_vldata_intro p min max)
 
@@ -367,7 +367,7 @@ let parse_vldata_intro_weak
   (min: U32.t)
   (max: U32.t { U32.v min <= U32.v max /\ U32.v max > 0 })
 : EWrite unit (parse_bounded_integer (log256 (max)) `star` p) (parse_vldata p min max) (fun _ -> True) (fun (_, vin) _ vout -> vin == vout) (fun (_, vin) -> ~ (U32.v min <= size p vin /\ size p vin <= U32.v max)) inv
-= EWrite?.reflect (| _, parse_vldata_intro_weak_impl p min max |)
+= EWrite?.reflect (Repr _ (parse_vldata_intro_weak_impl p min max))
 
 inline_for_extraction
 let parse_vldata_intro_weak_ho
@@ -388,7 +388,7 @@ let parse_vldata_intro_weak_ho
       begin match destr_repr_spec _ _ _ _ _ _ _ f () with
       | Correct (_, v) ->
         post () () v /\
-        (vout <: dfst p) == v
+        (vout <: Parser?.t p) == v
       | _ -> False
       end
     )
@@ -440,7 +440,7 @@ let parse_vldata_intro_weak_frame
   (p: parser)
   (min: U32.t)
   (max: U32.t { U32.v min <= U32.v max /\ U32.v max > 0 })
-: EWrite unit ((frame `star` parse_bounded_integer (log256 (max))) `star` p) (frame `star` parse_vldata p min max) (fun _ -> True) (fun ((fr, _), vin) _ (fr', vout) -> fr == fr' /\ (vin <: dfst p) == (vout <: dfst p)) (fun (_, vin) -> ~ (U32.v min <= size p vin /\ size p vin <= U32.v max)) inv
+: EWrite unit ((frame `star` parse_bounded_integer (log256 (max))) `star` p) (frame `star` parse_vldata p min max) (fun _ -> True) (fun ((fr, _), vin) _ (fr', vout) -> fr == fr' /\ (vin <: Parser?.t p) == (vout <: Parser?.t p)) (fun (_, vin) -> ~ (U32.v min <= size p vin /\ size p vin <= U32.v max)) inv
 = 
   valid_synth _ _ _ _ _ (valid_synth_star_assoc_1 _ _ _);
   frame2 _ _ _ _ _ _ _ _ (fun _ -> parse_vldata_intro_weak p min max)
@@ -451,7 +451,7 @@ let parse_vldata_recast_spec
   (max: U32.t { U32.v min <= U32.v max /\ U32.v max > 0 })
   (min': U32.t)
   (max': U32.t { U32.v min' <= U32.v max' /\ U32.v max' > 0 /\ log256 (max) == log256 (max')})
-: Tot (repr_spec unit (parse_vldata p min max) (parse_vldata p min' max') (fun _ -> True) (fun vin _ vout -> (vin <: dfst p) == (vout <: dfst p)) (fun vin -> ~ (U32.v min' <= size p vin /\ size p vin <= U32.v max')))
+: Tot (repr_spec unit (parse_vldata p min max) (parse_vldata p min' max') (fun _ -> True) (fun vin _ vout -> (vin <: Parser?.t p) == (vout <: Parser?.t p)) (fun vin -> ~ (U32.v min' <= size p vin /\ size p vin <= U32.v max')))
 =
   fun vin ->
     let sz = size p vin in
@@ -477,8 +477,8 @@ let parse_vldata_recast
   (max: U32.t { U32.v min <= U32.v max /\ U32.v max > 0 })
   (min': U32.t)
   (max': U32.t { U32.v min' <= U32.v max' /\ U32.v max' > 0 /\ log256 (max) == log256 (max')})
-: EWrite unit (parse_vldata p min max) (parse_vldata p min' max') (fun _ -> True) (fun vin _ vout -> (vin <: dfst p) == (vout <: dfst p)) (fun vin -> ~ (U32.v min' <= size p vin /\ size p vin <= U32.v max')) inv
-= EWrite?.reflect (| _, parse_vldata_recast_impl p min max min' max' |)
+: EWrite unit (parse_vldata p min max) (parse_vldata p min' max') (fun _ -> True) (fun vin _ vout -> (vin <: Parser?.t p) == (vout <: Parser?.t p)) (fun vin -> ~ (U32.v min' <= size p vin /\ size p vin <= U32.v max')) inv
+= EWrite?.reflect (Repr _ (parse_vldata_recast_impl p min max min' max'))
 
 inline_for_extraction
 type parser1 = (p: parser {
@@ -492,7 +492,7 @@ val valid_rlptr (p: parser1) : memory_invariant -> rlptr -> GTot Type0
 let lptr (p: parser1) (inv: memory_invariant) =
   (x: rlptr { valid_rlptr p inv x })
 
-val deref_list_spec (#p: parser1) (#inv: memory_invariant) (x: lptr p inv) : GTot (list (dfst p))
+val deref_list_spec (#p: parser1) (#inv: memory_invariant) (x: lptr p inv) : GTot (list (Parser?.t p))
 
 val valid_rlptr_frame
   (#p: parser1) (#inv: memory_invariant) (x: lptr p inv) (inv' : memory_invariant)
@@ -541,7 +541,7 @@ let destr_list
 let rec list_exists
   (#p: parser1)
   (#inv: memory_invariant)
-  (f_spec: Ghost.erased (dfst p -> Tot bool)) // reifying f below is not enough because of the ptr
+  (f_spec: Ghost.erased (Parser?.t p -> Tot bool)) // reifying f below is not enough because of the ptr
   (f: ((x: ptr p inv) -> Read bool (True) (fun res -> res == Ghost.reveal f_spec (deref_spec x)) inv))
   (l: lptr p inv)
 : Read bool (True) (fun res -> res == List.Tot.existsb f_spec (deref_list_spec l)) inv
@@ -555,7 +555,7 @@ let rec list_exists
 
 val list_size
   (p: parser1)
-  (x: list (dfst p))
+  (x: list (Parser?.t p))
 : GTot nat
 
 val list_size_nil
@@ -566,8 +566,8 @@ val list_size_nil
 
 val list_size_cons
   (p: parser1)
-  (a: dfst p)
-  (q: list (dfst p))
+  (a: Parser?.t p)
+  (q: list (Parser?.t p))
 : Lemma
   (list_size p (a :: q) == size p a + list_size p q)
   [SMTPat (list_size p (a :: q))]
@@ -576,7 +576,7 @@ module L = FStar.List.Tot
 
 let rec list_size_append
   (p: parser1)
-  (l1 l2: list (dfst p))
+  (l1 l2: list (Parser?.t p))
 : Lemma
   (list_size p (l1 `L.append` l2) == list_size p l1 + list_size p l2)
   [SMTPat (list_size p (l1 `L.append` l2))]
@@ -588,7 +588,7 @@ let parse_vllist_pred
   (p: parser1)
   (min: U32.t)
   (max: U32.t { U32.v min <= U32.v max /\ U32.v max > 0 })
-  (x: list (dfst p))
+  (x: list (Parser?.t p))
 : GTot Type0
 = let s = list_size p x in
   U32.v min <= s /\ s <= U32.v max
@@ -598,7 +598,7 @@ let parse_vllist_t
   (min: U32.t)
   (max: U32.t { U32.v min <= U32.v max /\ U32.v max > 0 })
 : Tot Type
-= (x: list (dfst p) { parse_vllist_pred p min max x })
+= (x: list (Parser?.t p) { parse_vllist_pred p min max x })
 
 inline_for_extraction
 val parse_vllist
@@ -606,7 +606,7 @@ val parse_vllist
   (min: U32.t)
   (max: U32.t { U32.v min <= U32.v max /\ U32.v max > 0 })
 : Tot (p' : parser {
-    dfst p' == parse_vllist_t p min max
+    Parser?.t p' == parse_vllist_t p min max
   })
 
 val parse_vllist_size
@@ -625,7 +625,7 @@ val lptr_of_vllist_ptr_repr
   (min: U32.t)
   (max: U32.t { U32.v min <= U32.v max /\ U32.v max > 0 })
   (r: ptr (parse_vllist p min max) inv)
-: Tot (read_repr (lptr p inv) True (fun r' -> deref_list_spec r' == (deref_spec r <: list (dfst p))) (fun _ -> False) inv)
+: Tot (read_repr (lptr p inv) True (fun r' -> deref_list_spec r' == (deref_spec r <: list (Parser?.t p))) (fun _ -> False) inv)
 
 inline_for_extraction
 let lptr_of_vllist_ptr
@@ -634,13 +634,13 @@ let lptr_of_vllist_ptr
   (min: U32.t)
   (max: U32.t { U32.v min <= U32.v max /\ U32.v max > 0 })
   (r: ptr (parse_vllist p min max) inv)
-: Read (lptr p inv) True (fun r' -> deref_list_spec r' == (deref_spec r <: list (dfst p))) inv
+: Read (lptr p inv) True (fun r' -> deref_list_spec r' == (deref_spec r <: list (Parser?.t p))) inv
 = ERead?.reflect (lptr_of_vllist_ptr_repr p min max r)
 
 let parse_vllist_nil_spec
   (p: parser1)
   (max: U32.t { U32.v max > 0 })
-: Tot (repr_spec unit emp (parse_vllist p 0ul max) (fun _ -> True) (fun _ _ x -> (x <: list (dfst p)) == [] /\ list_size p x == 0) (fun _ -> False))
+: Tot (repr_spec unit emp (parse_vllist p 0ul max) (fun _ -> True) (fun _ _ x -> (x <: list (Parser?.t p)) == [] /\ list_size p x == 0) (fun _ -> False))
 = fun _ ->
   Correct ((), ([] <: parse_vllist_t p 0ul max))
 
@@ -656,8 +656,8 @@ let parse_vllist_nil
   (#inv: memory_invariant)
   (p: parser1)
   (max: U32.t { U32.v max > 0 })
-: Write unit emp (parse_vllist p 0ul max) (fun _ -> True) (fun _ _ x -> (x <: list (dfst p)) == [] /\ list_size p x == 0) inv
-= EWrite?.reflect (| _, parse_vllist_nil_impl p max |)
+: Write unit emp (parse_vllist p 0ul max) (fun _ -> True) (fun _ _ x -> (x <: list (Parser?.t p)) == [] /\ list_size p x == 0) inv
+= EWrite?.reflect (Repr _ (parse_vllist_nil_impl p max))
 
 let parse_vllist_snoc_spec
   (p: parser1)
@@ -667,11 +667,11 @@ let parse_vllist_snoc_spec
     (fun (l, x) ->
       let sz = list_size p l + size p x in
       U32.v min <= sz /\ sz <= U32.v max)
-    (fun (l, x) _ l' -> (l' <: list (dfst p)) == L.snoc ((l <: list (dfst p)), x) /\ list_size p l' == list_size p l + size p x)
+    (fun (l, x) _ l' -> (l' <: list (Parser?.t p)) == L.snoc ((l <: list (Parser?.t p)), x) /\ list_size p l' == list_size p l + size p x)
     (fun _ -> False)
   )
 = fun (l, x) ->
-  Correct ((), L.snoc ((l <: list (dfst p)), x))
+  Correct ((), L.snoc ((l <: list (Parser?.t p)), x))
 
 inline_for_extraction
 val parse_vllist_snoc_impl
@@ -691,10 +691,10 @@ let parse_vllist_snoc
     (fun (l, x) ->
       let sz = list_size p l + size p x in
       U32.v min <= sz /\ sz <= U32.v max)
-    (fun (l, x) _ l' -> (l' <: list (dfst p)) == L.snoc ((l <: list (dfst p)), x) /\ list_size p l' == list_size p l + size p x)
+    (fun (l, x) _ l' -> (l' <: list (Parser?.t p)) == L.snoc ((l <: list (Parser?.t p)), x) /\ list_size p l' == list_size p l + size p x)
     inv
 =
-  EWrite?.reflect (| _, parse_vllist_snoc_impl p min max |)
+  EWrite?.reflect (Repr _ (parse_vllist_snoc_impl p min max))
 
 inline_for_extraction
 let parse_vllist_snoc_ho
@@ -720,7 +720,7 @@ let parse_vllist_snoc_ho
       begin match destr_repr_spec _ _ _ _ _ _ _ f () with
       | Correct (_, v) ->
         post () () v /\
-        (vout <: list (dfst p)) == (vin <: list (dfst p)) `L.append` [v]
+        (vout <: list (Parser?.t p)) == (vin <: list (Parser?.t p)) `L.append` [v]
       | _ -> False
       end
     )
@@ -750,7 +750,7 @@ let parse_vllist_snoc_ho'
     (fun vin _ vout ->
       begin match destr_repr_spec _ _ _ _ _ _ _ f () with
       | Correct (_, v) ->
-        (vout <: list (dfst p)) == (vin <: list (dfst p)) `L.append` [v]
+        (vout <: list (Parser?.t p)) == (vin <: list (Parser?.t p)) `L.append` [v]
       | _ -> False
       end
     )
@@ -768,7 +768,7 @@ let parse_vllist_snoc_weak_spec
   (max: U32.t { U32.v min <= U32.v max /\ U32.v max > 0 })
 : Tot (repr_spec unit (parse_vllist p min max `star` p) (parse_vllist p min max)
     (fun _ -> True)
-    (fun (l, x) _ l' -> (l' <: list (dfst p)) == L.snoc ((l <: list (dfst p)), x) /\ list_size p l' == list_size p l + size p x)
+    (fun (l, x) _ l' -> (l' <: list (Parser?.t p)) == L.snoc ((l <: list (Parser?.t p)), x) /\ list_size p l' == list_size p l + size p x)
     (fun (l, x) ->
       let sz = list_size p l + size p x in
       ~ (U32.v min <= sz /\ sz <= U32.v max))
@@ -777,7 +777,7 @@ let parse_vllist_snoc_weak_spec
   let sz = list_size p l + size p x in
   if U32.v min <= sz && sz <= U32.v max
   then begin
-    Correct ((), L.snoc ((l <: list (dfst p)), x))
+    Correct ((), L.snoc ((l <: list (Parser?.t p)), x))
   end else
     Error "parse_vllist_snoc_weak: out of bounds"
 
@@ -797,13 +797,13 @@ let parse_vllist_snoc_weak
   (max: U32.t { U32.v min <= U32.v max /\ U32.v max > 0 })
 : EWrite unit (parse_vllist p min max `star` p) (parse_vllist p min max)
     (fun _ -> True)
-    (fun (l, x) _ l' -> (l' <: list (dfst p)) == L.snoc ((l <: list (dfst p)), x) /\ list_size p l' == list_size p l + size p x)
+    (fun (l, x) _ l' -> (l' <: list (Parser?.t p)) == L.snoc ((l <: list (Parser?.t p)), x) /\ list_size p l' == list_size p l + size p x)
     (fun (l, x) ->
       let sz = list_size p l + size p x in
       ~ (U32.v min <= sz /\ sz <= U32.v max))
     inv
 =
-  EWrite?.reflect (| _, parse_vllist_snoc_weak_impl p min max |)
+  EWrite?.reflect (Repr _ (parse_vllist_snoc_weak_impl p min max))
 
 inline_for_extraction
 let parse_vllist_snoc_weak_ho
@@ -824,7 +824,7 @@ let parse_vllist_snoc_weak_ho
       begin match destr_repr_spec _ _ _ _ _ _ _ f () with
       | Correct (_, v) ->
         post () () v /\
-        (vout <: list (dfst p)) == (vin <: list (dfst p)) `L.append` [v]
+        (vout <: list (Parser?.t p)) == (vin <: list (Parser?.t p)) `L.append` [v]
       | _ -> False
       end
     )
@@ -854,7 +854,7 @@ let parse_vllist_snoc_weak_ho'
     (fun vin _ vout ->
       begin match destr_repr_spec _ _ _ _ _ _ _ f () with
       | Correct (_, v) ->
-        (vout <: list (dfst p)) == (vin <: list (dfst p)) `L.append` [v]
+        (vout <: list (Parser?.t p)) == (vin <: list (Parser?.t p)) `L.append` [v]
       | _ -> False
       end
     )
@@ -885,7 +885,7 @@ let parse_vllist_recast_spec
   (max: U32.t { U32.v min <= U32.v max /\ U32.v max > 0 })
   (min': U32.t)
   (max': U32.t { U32.v min' <= U32.v max' /\ U32.v max' > 0 /\ log256 max == log256 (max')})
-: Tot (repr_spec unit (parse_vllist p min max) (parse_vllist p min' max') (fun _ -> True) (fun vin _ vout -> (vin <: list (dfst p)) == (vout <: list (dfst p))) (fun vin -> ~ (U32.v min' <= list_size p vin /\ list_size p vin <= U32.v max')))
+: Tot (repr_spec unit (parse_vllist p min max) (parse_vllist p min' max') (fun _ -> True) (fun vin _ vout -> (vin <: list (Parser?.t p)) == (vout <: list (Parser?.t p))) (fun vin -> ~ (U32.v min' <= list_size p vin /\ list_size p vin <= U32.v max')))
 =
   fun vin ->
     let sz = list_size p vin in
@@ -911,8 +911,8 @@ let parse_vllist_recast
   (max: U32.t { U32.v min <= U32.v max /\ U32.v max > 0 })
   (min': U32.t)
   (max': U32.t { U32.v min' <= U32.v max' /\ U32.v max' > 0 /\ log256 (max) == log256 (max')})
-: EWrite unit (parse_vllist p min max) (parse_vllist p min' max') (fun _ -> True) (fun vin _ vout -> (vin <: list (dfst p)) == (vout <: list (dfst p))) (fun vin -> ~ (U32.v min' <= list_size p vin /\ list_size p vin <= U32.v max')) inv
-= EWrite?.reflect (| _, parse_vllist_recast_impl p min max min' max' |)
+: EWrite unit (parse_vllist p min max) (parse_vllist p min' max') (fun _ -> True) (fun vin _ vout -> (vin <: list (Parser?.t p)) == (vout <: list (Parser?.t p))) (fun vin -> ~ (U32.v min' <= list_size p vin /\ list_size p vin <= U32.v max')) inv
+= EWrite?.reflect (Repr _ (parse_vllist_recast_impl p min max min' max'))
 
 let parse_vlbytes_pred
   (min: nat)
@@ -933,7 +933,7 @@ val parse_vlbytes
   (min: U32.t)
   (max: U32.t { U32.v min <= U32.v max /\ U32.v max > 0 })
 : Tot (p' : parser {
-    dfst p' == parse_vlbytes_t (U32.v min) (U32.v max)
+    Parser?.t p' == parse_vlbytes_t (U32.v min) (U32.v max)
   })
 
 module B = LowStar.Buffer
@@ -1004,12 +1004,12 @@ let put_vlbytes
   (l: Ghost.erased (Seq.seq LP.byte) { Seq.length l == U32.v len })
   (f: put_vlbytes_impl_t inv min max len l)
 : Write unit emp (parse_vlbytes min max) (fun _ -> True) (fun _ _ vout -> vout == FStar.Bytes.hide (Ghost.reveal l)) inv
-= EWrite?.reflect (| _, put_vlbytes_impl min max len l f |)
+= EWrite?.reflect (Repr _ (put_vlbytes_impl min max len l f))
 
 let rec list_map'
   (p1 p2: parser1)
   (#inv: memory_invariant)
-  (f: Ghost.erased (dfst p1 -> Tot (dfst p2)))
+  (f: Ghost.erased (Parser?.t p1 -> Tot (Parser?.t p2)))
   (f' : (
     (x: ptr p1 inv) ->
     Write unit emp p2 (fun _ -> True) (fun _ _ out -> out == Ghost.reveal f (deref_spec x)) inv
@@ -1022,7 +1022,7 @@ let rec list_map'
     (parse_vllist p2 min max)
     (parse_vllist p2 min max)
     (fun _ -> True)
-    (fun lin _ lout -> (lout <: list (dfst p2)) == (lin <: list (dfst p2)) `L.append` L.map (Ghost.reveal f) (deref_list_spec l))
+    (fun lin _ lout -> (lout <: list (Parser?.t p2)) == (lin <: list (Parser?.t p2)) `L.append` L.map (Ghost.reveal f) (deref_list_spec l))
     (fun lin -> list_size p2 lin + list_size p2 (L.map (Ghost.reveal f) (deref_list_spec l)) > U32.v max)
     inv
   (decreases (deref_list_spec l))
@@ -1030,7 +1030,7 @@ let rec list_map'
   let lin = get_state () in
   match destr_list l with
   | None ->
-    L.append_l_nil (Ghost.reveal lin <: list (dfst p2))
+    L.append_l_nil (Ghost.reveal lin <: list (Parser?.t p2))
   | Some (hd, tl) ->
     frame _ _ _ _ _ _ _ (fun _ -> f' hd);
     parse_vllist_snoc_weak p2 min max;
@@ -1040,7 +1040,7 @@ let rec list_map'
 let list_map
   (p1 p2: parser1)
   (#inv: memory_invariant)
-  (f: Ghost.erased (dfst p1 -> Tot (dfst p2)))
+  (f: Ghost.erased (Parser?.t p1 -> Tot (Parser?.t p2)))
   (f' : (
     (x: ptr p1 inv) ->
     Write unit emp p2 (fun _ -> True) (fun _ _ out -> out == Ghost.reveal f (deref_spec x)) inv
@@ -1053,7 +1053,7 @@ let list_map
     emp
     (parse_vllist p2 min max)
     (fun _ -> True)
-    (fun _ _ lout -> (lout <: list (dfst p2)) == L.map (Ghost.reveal f) (deref_list_spec l))
+    (fun _ _ lout -> (lout <: list (Parser?.t p2)) == L.map (Ghost.reveal f) (deref_list_spec l))
     (fun _ -> let len = list_size p2 (L.map (Ghost.reveal f) (deref_list_spec l)) in len < U32.v min \/ len > U32.v max)
     inv
 =
@@ -1066,7 +1066,7 @@ let list_map
 inline_for_extraction
 noextract
 val parse_u32 : (p': parser {
-  dfst p' == U32.t /\
+  Parser?.t p' == U32.t /\
   get_parser_kind p' == LPI.parse_u32_kind /\
   get_parser p' == LPI.parse_u32 /\
   get_serializer p' == LPI.serialize_u32
@@ -1075,7 +1075,7 @@ val parse_u32 : (p': parser {
 inline_for_extraction
 noextract
 val parse_u16 : (p': parser {
-  dfst p' == FStar.UInt16.t /\
+  Parser?.t p' == FStar.UInt16.t /\
   get_parser_kind p' == LPI.parse_u16_kind /\
   get_parser p' == LPI.parse_u16 /\
   get_serializer p' == LPI.serialize_u16
@@ -1084,7 +1084,7 @@ val parse_u16 : (p': parser {
 inline_for_extraction
 noextract
 val parse_u8 : (p': parser {
-  dfst p' == FStar.UInt8.t /\
+  Parser?.t p' == FStar.UInt8.t /\
   get_parser_kind p' == LPI.parse_u8_kind /\
   get_parser p' == LPI.parse_u8 /\
   get_serializer p' == LPI.serialize_u8
