tests/layeff/LowParseWriters.LowParse.fst
@@ -23,7 +23,7 @@ let slice_of_buffer
 
 let valid_pos
   p h b pos pos'
-= LP.valid_pos (dsnd p).parser h (slice_of_buffer b) pos pos'
+= LP.valid_pos (Parser?.p p).parser h (slice_of_buffer b) pos pos'
 
 let valid_pos_post
   p h b pos pos'
@@ -32,16 +32,16 @@ let valid_pos_post
 let contents
   p h b pos pos'
 =
-  LP.contents (dsnd p).parser h (slice_of_buffer b) pos
+  LP.contents (Parser?.p p).parser h (slice_of_buffer b) pos
 
 let size
   p x
-= Seq.length (LP.serialize (dsnd p).serializer x)
+= Seq.length (LP.serialize (Parser?.p p).serializer x)
 
 let contents_size
   p h b pos pos'
-= LP.valid_pos_valid_exact (dsnd p).parser h (slice_of_buffer b) pos pos';
-  LP.valid_exact_serialize (dsnd p).serializer h (slice_of_buffer b) pos pos'
+= LP.valid_pos_valid_exact (Parser?.p p).parser h (slice_of_buffer b) pos pos';
+  LP.valid_exact_serialize (Parser?.p p).serializer h (slice_of_buffer b) pos pos'
 
 let emp' = {
   kind = _;
@@ -69,19 +69,19 @@ let star'
 let valid_star
   p1 p2 h b pos1 pos2 pos3
 =
-  LP.valid_nondep_then h (dsnd p1).parser (dsnd p2).parser (slice_of_buffer b) pos1
+  LP.valid_nondep_then h (Parser?.p p1).parser (Parser?.p p2).parser (slice_of_buffer b) pos1
 
 let size_star
   p1 p2 x1 x2
 =
-  LP.length_serialize_nondep_then (dsnd p1).serializer (dsnd p2).serializer x1 x2
+  LP.length_serialize_nondep_then (Parser?.p p1).serializer (Parser?.p p2).serializer x1 x2
 
 let valid_ext
   p h1 b1 pos1 pos1' h2 b2 pos2 pos2'
 =
   assert (Seq.length (B.as_seq h2 (B.gsub b2 pos2 (pos2' `U32.sub` pos2))) == Seq.length (B.as_seq h1 (B.gsub b1 pos1 (pos1' `U32.sub` pos1))));
   assert (pos2' `U32.sub` pos2 == pos1' `U32.sub` pos1);
-  LP.valid_ext_intro (dsnd p).parser h1 (LP.make_slice b1 (B.len b1)) pos1 h2 (LP.make_slice b2 (B.len b2)) pos2
+  LP.valid_ext_intro (Parser?.p p).parser h1 (LP.make_slice b1 (B.len b1)) pos1 h2 (LP.make_slice b2 (B.len b2)) pos2
 
 let parse_u32' = {
   kind = _;
@@ -100,15 +100,15 @@ let valid_star_inv_spec
   h p1 p2 b pos1 pos3
 =
   let sl = LP.make_slice b (B.len b) in
-  LP.valid_nondep_then h (dsnd p1).parser (dsnd p2).parser sl pos1;
-  LP.get_valid_pos (dsnd p1).parser h sl pos1
+  LP.valid_nondep_then h (Parser?.p p1).parser (Parser?.p p2).parser sl pos1;
+  LP.get_valid_pos (Parser?.p p1).parser h sl pos1
 
 let valid_star_inv
   p1 p2 b len pos1 pos3
 =
   let h = HST.get () in
-  LP.valid_nondep_then h (dsnd p1).parser (dsnd p2).parser (LP.make_slice b len) pos1;
-  (dsnd p1).jumper (LP.make_slice b len) pos1
+  LP.valid_nondep_then h (Parser?.p p1).parser (Parser?.p p2).parser (LP.make_slice b len) pos1;
+  (Parser?.p p1).jumper (LP.make_slice b len) pos1
 
 let clens_to_lp_clens
   (#t1 #t2: Type)
@@ -121,30 +121,31 @@ let clens_to_lp_clens
 
 let gaccessor
   p1 p2 lens
-= LP.gaccessor (dsnd p1).parser (dsnd p2).parser (clens_to_lp_clens lens)
+= LP.gaccessor (Parser?.p p1).parser (Parser?.p p2).parser (clens_to_lp_clens lens)
 
-#push-options "--z3rlimit 16"
+#push-options "--z3rlimit 32"
+#restart-solver
 
 let gaccess
   #p1 #p2 #lens g h b
 =
   let sl = LP.make_slice b (B.len b) in
-  LP.valid_facts (dsnd p1).parser h sl 0ul;
+  LP.valid_facts (Parser?.p p1).parser h sl 0ul;
   let posn = g (B.as_seq h b) in
   let pos = U32.uint_to_t posn in
-  LP.valid_facts (dsnd p2).parser h sl pos;
-  let pos' = LP.get_valid_pos (dsnd p2).parser h sl pos in
+  LP.valid_facts (Parser?.p p2).parser h sl pos;
+  let pos' = LP.get_valid_pos (Parser?.p p2).parser h sl pos in
   let b1 = B.gsub b pos (B.len b `U32.sub` pos) in
   let len' = pos' `U32.sub` pos in
   let b' = B.gsub b1 0ul len' in
-  LP.parse_strong_prefix (dsnd p2).parser (B.as_seq h b1) (B.as_seq h b');
+  LP.parse_strong_prefix (Parser?.p p2).parser (B.as_seq h b1) (B.as_seq h b');
   let sl' = LP.make_slice b' (B.len b') in
-  LP.valid_facts (dsnd p2).parser h sl' 0ul;
+  LP.valid_facts (Parser?.p p2).parser h sl' 0ul;
   b'
 
 let gaccessor_frame1
   (#p1 #p2: parser)
-  (#lens: clens (dfst p1) (dfst p2))
+  (#lens: clens (Parser?.t p1) (Parser?.t p2))
   (g: gaccessor p1 p2 lens)
   (h: HS.mem)
   (b: B.buffer u8)
@@ -168,17 +169,17 @@ let gaccessor_frame1
     gaccess g h' b == gaccess g h b
   ))
 = let sl = LP.make_slice b (B.len b) in
-  LP.valid_facts (dsnd p1).parser h sl 0ul;
+  LP.valid_facts (Parser?.p p1).parser h sl 0ul;
   let posn = g (B.as_seq h b) in
   let pos = U32.uint_to_t posn in
-  LP.valid_facts (dsnd p2).parser h sl pos;
-  let pos' = LP.get_valid_pos (dsnd p2).parser h sl pos in
+  LP.valid_facts (Parser?.p p2).parser h sl pos;
+  let pos' = LP.get_valid_pos (Parser?.p p2).parser h sl pos in
   let b1 = B.gsub b pos (B.len b `U32.sub` pos) in
   let len' = pos' `U32.sub` pos in
   let b' = B.gsub b1 0ul len' in
-  LP.parse_strong_prefix (dsnd p2).parser (B.as_seq h b1) (B.as_seq h b');
+  LP.parse_strong_prefix (Parser?.p p2).parser (B.as_seq h b1) (B.as_seq h b');
   let sl' = LP.make_slice b' (B.len b') in
-  LP.valid_facts (dsnd p2).parser h sl' 0ul;
+  LP.valid_facts (Parser?.p p2).parser h sl' 0ul;
   ()
 
 #pop-options
@@ -199,16 +200,16 @@ let baccess
 =
   let h = HST.get () in
   let sl = LP.make_slice b len in
-  LP.valid_facts (dsnd p1).parser h sl 0ul;
+  LP.valid_facts (Parser?.p p1).parser h sl 0ul;
   let pos = a sl 0ul in
   LP.slice_access_eq h g sl 0ul;
-  LP.valid_facts (dsnd p2).parser h sl pos;
-  let pos' = (dsnd p2).jumper sl pos in
+  LP.valid_facts (Parser?.p p2).parser h sl pos;
+  let pos' = (Parser?.p p2).jumper sl pos in
   let b1 = B.sub b pos (B.len b `U32.sub` pos) in
   let len' = pos' `U32.sub` pos in
   let b' = B.sub b1 0ul len' in
-  LP.parse_strong_prefix (dsnd p2).parser (B.as_seq h b1) (B.as_seq h b');
-  LP.valid_facts (dsnd p2).parser h (LP.make_slice b' (B.len b')) 0ul;
+  LP.parse_strong_prefix (Parser?.p p2).parser (B.as_seq h b1) (B.as_seq h b');
+  LP.valid_facts (Parser?.p p2).parser h (LP.make_slice b' (B.len b')) 0ul;
   (b', len')
 
 #pop-options
@@ -217,11 +218,11 @@ let validator
   p
 =
   (
-    squash begin match (dsnd p).kind.LP.parser_kind_high with
+    squash begin match (Parser?.p p).kind.LP.parser_kind_high with
     | None -> False
     | Some max -> max <= U32.v LP.validator_max_length
     end &
-    LP.validator (dsnd p).parser
+    LP.validator (Parser?.p p).parser
   )
 
 inline_for_extraction
@@ -231,8 +232,8 @@ let gvalidate
   p h b
 =
   let sl = LP.make_slice b (B.len b) in
-  LP.valid_facts (dsnd p).parser h sl 0ul;
-  match LP.parse (dsnd p).parser (B.as_seq h b) with
+  LP.valid_facts (Parser?.p p).parser h sl 0ul;
+  match LP.parse (Parser?.p p).parser (B.as_seq h b) with
   | None -> None
   | Some (_, res) -> Some (U32.uint_to_t res)
 
